ArkLib.lean
@@ -291,6 +291,7 @@ import ArkLib.OracleReduction.Composition.Sequential.Append
 import ArkLib.OracleReduction.Composition.Sequential.Append.Basic
 import ArkLib.OracleReduction.Composition.Sequential.Append.Execution
 import ArkLib.OracleReduction.Composition.Sequential.Append.Security
+import ArkLib.OracleReduction.Composition.Sequential.Append.Simulation
 import ArkLib.OracleReduction.Composition.Sequential.Append.StateFunction
 import ArkLib.OracleReduction.Composition.Sequential.General
 import ArkLib.OracleReduction.Composition.Sequential.IsPure
